\subsubsection{Extension 2}
\begin{namedframe}{On the major arc}
	\begin{example}
		Show that the Star Trek theorem is still true if $\angle AOB > \SI{180}{\degree}$.
		\vertspace
		That is, show that $\angle AOB = 2\angle ACB$ is true in this diagram.
	\end{example}
	\centering
	\begin{tikzpicture}[scale=0.4]
		\coordinate [label=below:$O$](O) at (0,0);
		\coordinate [label=below left:$A$](A) at (-5,0);
		\coordinate [label=below right:$B$](B) at (4.75,1.5612494996);
		\coordinate [label=above left:$C$](C) at (-1,4.89897948557);

		\draw (O) circle (5);
		\draw (A) -- (O) -- (B) -- (C) -- cycle;
		\draw [dashed] (O) -- (C);

		\pic [draw, "$\angle BOA$", angle eccentricity=1.5] {angle = B--O--A};
		\pic [draw, "$\angle AOB$", angle eccentricity=1.5, angle radius=6mm] {angle = A--O--B};
	\end{tikzpicture}
\end{namedframe}
\begin{namedframe}{Extension 2 proof}
	\footnotesize
	\begin{proof}[Proof that $\angle AOB = 2\angle ACB $.]
		\vspace{-2ex}
		\begin{wrapfigure}[0]{r}{0pt}
			\scriptsize
			\begin{tikzpicture}[scale=0.2]
				\coordinate [label=below:$O$](O) at (0,0);
				\coordinate [label=below left:$A$](A) at (-5,0);
				\coordinate [label=below right:$B$](B) at (4.75,1.5612494996);
				\coordinate [label=above left:$C$](C) at (-1,4.89897948557);

				\draw (O) circle (5);
				\draw (A) -- (O) -- (B) -- (C) -- cycle;
				\draw [dashed] (O) -- (C);

				\pic [draw, "$\angle BOA$", angle eccentricity=1.5, angle radius=3mm] {angle = B--O--A};
				\pic [draw, "$\angle AOB$", angle eccentricity=1.5, angle radius=4mm] {angle = A--O--B};
			\end{tikzpicture}
		\end{wrapfigure}
		\[2\angle ACO + \angle AOC = \SI{180}{\degree}\]
		\[2\angle BCO + \angle BOC = \SI{180}{\degree}\]
		\sep
		We add these two equations to get:
		\sep[0pt]
		\begin{align*}
			2(\angle ACO + \angle BCO) + \angle AOC + \angle BOC &= \SI{360}{\degree}\\
			2(\angle ACO + \angle BCO) &= \SI{360}{\degree} - (\angle AOC + \angle BOC)
		\end{align*}
		\pause
		We know that $\angle AOC + \angle BOC = \angle BOA$, so:
		\[2(\angle ACO + \angle BCO) = \SI{360}{\degree} - \angle BOA\]
		\pause
		We also know that $\angle AOB = \SI{360}{\degree} - \angle BOA$.
		\sep[0pt]
		And $\angle ACB = \angle ACO + \angle BOC$.
		\pause
		\[\therefore 2\angle ACB = \angle AOB \qedhere\]
	\end{proof}
\end{namedframe}
